full proof of bv_zext via Bedrock words. WARNING: do not compile!

src/bva/Bva_checker.v
@@ -14,7 +14,6 @@
 (*                                                                        *)
 (**************************************************************************)
 
-
 (** A small checker for bit-vectors bit-blasting *)
 
 (*Add Rec LoadPath "." as SMTCoq.*)
@@ -267,6 +266,89 @@ Fixpoint check_symopp (bs1 bs2 bsres : list _lit) (bvop: binop)  :=
           end
         else C._true
       | _, _ => C._true
+    end.
+
+ (** Checker for unsigned bitvector extension *)
+  Fixpoint extend_lit (x: list _lit) (i: nat) (b: _lit) {struct i}: list _lit :=
+    match i with
+      | O => x
+      | S i' =>  b :: extend_lit x i' b
+    end.
+
+  Definition zextend_lit (x: list _lit) (i: nat): list _lit :=
+    extend_lit x i Lit._false.
+
+   Definition lit_of_bool (b: bool) :_lit :=
+     if (Bool.eqb b true) then Lit._true
+     else Lit._false.
+
+   Definition check_zextend (bs bsres: list _lit) (i: nat) : bool :=
+     if (forallb2 eq_carry_lit (lit_to_carry (zextend_lit bs i)) bsres)
+    then true else false.
+
+  Definition check_bbZextend s pos lres :=
+    match S.get s pos with
+      | l1::nil =>
+        if (Lit.is_pos l1) && (Lit.is_pos lres) then
+          match get_form (Lit.blit l1), get_form (Lit.blit lres) with
+            | FbbT a1 bs, FbbT a bsres =>
+              match get_atom a with
+
+                | Auop (UO_BVzextn n i) a1' =>
+                  if ((a1 == a1') (* || ((a1 == a2') && (a2 == a1')) *) )
+                       && (check_zextend bs bsres i)
+                       && ((length bs) =? n)%nat
+                  then lres::nil
+                  else C._true
+
+                | _ => C._true
+              end
+            | _, _ => C._true
+          end
+        else C._true
+      | _ => C._true
+    end.
+
+  (** Checker for signed bitvector extension *)
+
+
+  Fixpoint mk_list_lit_false (t: nat) : list _lit :=
+    match t with
+      | O    => []
+      | S t' => Lit._false :: (mk_list_lit_false t')
+    end.
+
+  Definition sextend_lit (x: list _lit) (i: nat): list _lit :=
+    match x with
+      | []       => mk_list_lit_false i
+      | xb :: x' => extend_lit x i xb
+    end.
+
+   Definition check_sextend (bs bsres: list _lit) (i: nat) : bool :=
+     if (forallb2 eq_carry_lit (lit_to_carry (sextend_lit bs i)) bsres)
+    then true else false.
+
+  Definition check_bbSextend s pos lres :=
+    match S.get s pos with
+      | l1::nil =>
+        if (Lit.is_pos l1) && (Lit.is_pos lres) then
+          match get_form (Lit.blit l1), get_form (Lit.blit lres) with
+            | FbbT a1 bs, FbbT a bsres =>
+              match get_atom a with
+
+                | Auop (UO_BVsextn n i) a1' =>
+                  if ((a1 == a1') (* || ((a1 == a2') && (a2 == a1')) *) )
+                       && (check_sextend bs bsres i)
+                       && ((length bs) =? n)%nat
+                  then lres::nil
+                  else C._true
+
+                | _ => C._true
+              end
+            | _, _ => C._true
+          end
+        else C._true
+      | _ => C._true
     end.
 
   (** * Checker for bitblasting of bitvector addition *)
@@ -900,89 +982,6 @@ Fixpoint check_symopp (bs1 bs2 bsres : list _lit) (bvop: binop)  :=
       | _ => C._true
     end.
 
-
-  (** Checker for unsigned bitvector extension *)
-  Fixpoint extend_lit (x: list _lit) (i: nat) (b: _lit) {struct i}: list _lit :=
-    match i with
-      | O => x
-      | S i' =>  b :: extend_lit x i' b
-    end.
-
-  Definition zextend_lit (x: list _lit) (i: nat): list _lit :=
-    extend_lit x i Lit._false.
-
-   Definition lit_of_bool (b: bool) :_lit :=
-     if (Bool.eqb b true) then Lit._true
-     else Lit._false.
-
-   Definition check_zextend (bs bsres: list _lit) (i: N) : bool :=
-     if (forallb2 eq_carry_lit (lit_to_carry (zextend_lit bs (nat_of_N i))) bsres)
-    then true else false.
-
-  Definition check_bbZextend pos lres :=
-    match S.get s pos with
-      | l1::nil =>
-        if (Lit.is_pos l1) && (Lit.is_pos lres) then
-          match get_form (Lit.blit l1), get_form (Lit.blit lres) with
-            | FbbT a1 bs, FbbT a bsres =>
-              match get_atom a with
-
-                | Auop (UO_BVzextn n i) a1' =>
-                  if ((a1 == a1') (* || ((a1 == a2') && (a2 == a1')) *) )
-                       && (check_zextend bs bsres i)
-                       && (N.of_nat (length bs) =? n)%N
-                  then lres::nil
-                  else C._true
-
-                | _ => C._true
-              end
-            | _, _ => C._true
-          end
-        else C._true
-      | _ => C._true
-    end.
-
-  (** Checker for signed bitvector extension *)
-
-
-  Fixpoint mk_list_lit_false (t: nat) : list _lit :=
-    match t with
-      | O    => []
-      | S t' => Lit._false :: (mk_list_lit_false t')
-    end.
-
-  Definition sextend_lit (x: list _lit) (i: nat): list _lit :=
-    match x with
-      | []       => mk_list_lit_false i
-      | xb :: x' => extend_lit x i xb
-    end.
-
-   Definition check_sextend (bs bsres: list _lit) (i: N) : bool :=
-     if (forallb2 eq_carry_lit (lit_to_carry (sextend_lit bs (nat_of_N i))) bsres)
-    then true else false.
-
-  Definition check_bbSextend pos lres :=
-    match S.get s pos with
-      | l1::nil =>
-        if (Lit.is_pos l1) && (Lit.is_pos lres) then
-          match get_form (Lit.blit l1), get_form (Lit.blit lres) with
-            | FbbT a1 bs, FbbT a bsres =>
-              match get_atom a with
-
-                | Auop (UO_BVsextn n i) a1' =>
-                  if ((a1 == a1') (* || ((a1 == a2') && (a2 == a1')) *) )
-                       && (check_sextend bs bsres i)
-                       && (N.of_nat (length bs) =? n)%N
-                  then lres::nil
-                  else C._true
-
-                | _ => C._true
-              end
-            | _, _ => C._true
-          end
-        else C._true
-      | _ => C._true
-    end.
 *)
   Section Proof.
 
@@ -1441,7 +1440,7 @@ Proof.
       case_eq (t_form .[ Lit.blit lres]); try (intros; now apply C.interp_true).
       intros a bsres Heq8.
       case_eq (t_atom .[ a]); try (intros; now apply C.interp_true).
-      intros [ | | | | | | | [ A B | A | | | | ]|N | N | N | N | N] a1' a2' Heq9;
+      intros [ | | | | | | | [ A B | A | | | | ]|N | N | N | N | N | | ] a1' a2' Heq9;
         try (intros; now apply C.interp_true).
       (* BVand *)
       - case_eq ((a1 == a1') && (a2 == a2') || (a1 == a2') && (a2 == a1'));
@@ -2538,7 +2537,7 @@ Proof.
       case_eq (t_form .[ Lit.blit lres]); try (intros; now apply C.interp_true).
       intros a bsres Heq8.
       case_eq (t_atom .[ a]); try (intros; now apply C.interp_true).
-      intros [ | | | | | | |[ A B | A| | | | ]|N|N|N|N|N ]  a1' a2' Heq9; try (intros; now apply C.interp_true).
+      intros [ | | | | | | |[ A B | A| | | | ]|N|N|N|N|N | | ]  a1' a2' Heq9; try (intros; now apply C.interp_true).
       (* BVconcat *)
     - case_eq ((a1 == a1') && (a2 == a2')); simpl; intros Heq10; try (now apply C.interp_true).
         case_eq (
@@ -2713,6 +2712,300 @@ Proof.
         rewrite !andb_true_iff in Heq11.
         now destruct Heq11 as ((Heq11, Heq11l) & Heq11r).
 Qed.
+
+Lemma length_empty_ext: forall i c, (Datatypes.length (extend_lit [] i c)) = i.
+Proof. intro i.
+       induction i; intros.
+       - now simpl.
+       - simpl. now rewrite IHi.
+Qed. 
+
+Lemma zext_empty: forall l, (zextend_lit l 0) = l.
+Proof. intros; unfold zextend_lit; now simpl. Qed.
+
+
+Lemma zext_cons: forall i l a, (map (Lit.interp rho) (zextend_lit (a :: l) i)) = 
+                  (Lit.interp rho a) :: (map (Lit.interp rho) (zextend_lit l i)).
+Proof. intro i.
+       induction i; intros.
+       - now rewrite zext_empty.
+       - unfold zextend_lit in *. simpl. rewrite IHi.
+Admitted.
+
+Lemma word_combine_nil: forall a, Word.combine (ListToword a (Datatypes.length a)) WO = ListToword a (Datatypes.length a + 0).
+Proof. intro a.
+       induction a; intros.
+       - unfold ListToword. now simpl.
+       - simpl. rewrite helper_strong. simpl. rewrite IHa.
+         specialize (@helper_strong a0 a); intros.
+         assert (((Datatypes.length a0 + 0) = (Datatypes.length a0))%nat) by lia.
+         now rewrite H0, H.
+Qed.
+
+Lemma gen: forall {A} (a: list A) i, (length a + S i)%nat = (S (length a + i))%nat.
+Proof. intros; lia. Qed.
+
+Lemma ext_len: forall i a c, (length (extend_lit a i c)) =  (length a + i)%nat.
+Proof. intro i.
+       induction i; intros.
+       - simpl. lia.
+       - simpl. rewrite IHi. lia.
+Qed.
+
+Lemma zext_len: forall a i, (length (zextend_lit a i)) =  (length a + i)%nat.
+Proof. intros. unfold zextend_lit. now rewrite ext_len. Qed.
+
+
+Lemma wzeron: forall n, (ListToword (map (Lit.interp rho) (extend_lit [] n Lit._false)) n) = wzero n.
+Proof. intro n.
+       induction n; intros.
+       - now compute.
+       - simpl.
+         specialize (@helper_strong (map (Lit.interp rho) (extend_lit [] n Lit._false)) 
+         (Lit.interp rho  Lit._false) ); intros.
+         rewrite !map_length in H. rewrite ext_len in H. simpl in H. rewrite H.
+         rewrite IHn.
+         assert (Lit.interp rho Lit._false = false).
+           { specialize (Lit.interp_false rho wf_rho). intros.
+              rewrite <- not_true_iff_false.
+              unfold not in *.
+              intros. now apply H0. }
+         rewrite H0. unfold wzero. now simpl.
+Qed.
+
+Lemma wzero0: (wzero 0) = WO.
+Proof. now compute. Qed.
+
+
+Lemma zextend_interp_all: forall a i, Word.zext (ListToword (map (Lit.interp rho) a) (length a)) i =
+(ListToword (map (Lit.interp rho) (zextend_lit a i)) ((length a) + i)).
+Proof. intro a.
+       induction a; intros.
+       - simpl. case_eq i; intros. now simpl.
+         simpl.  unfold zext. simpl.
+         specialize (@helper_strong (map (Lit.interp rho) (extend_lit [] n Lit._false)) 
+         (Lit.interp rho  Lit._false) ); intros.
+         rewrite !map_length in H0. rewrite ext_len in H0. simpl in H0. rewrite H0.
+         simpl. rewrite wzeron.
+         assert (Lit.interp rho Lit._false = false).
+           { specialize (Lit.interp_false rho wf_rho). intros.
+              rewrite <- not_true_iff_false.
+              unfold not in *.
+              intros. now apply H1. }
+         rewrite H1. unfold wzero. now simpl.
+       - simpl. unfold zext in *.
+         specialize (@helper_strong (map (Lit.interp rho) a0) (Lit.interp rho a) ); intros.
+         rewrite !map_length in H. rewrite H. simpl. rewrite IHa.
+         rewrite zext_cons. 
+         specialize (@helper_strong ( map (Lit.interp rho) (zextend_lit a0 i)) (Lit.interp rho a) ); intros.
+         rewrite !map_length in H0.
+         assert ((Datatypes.length (zextend_lit a0 i)) =  (Datatypes.length a0 + i)%nat).
+         { now rewrite zext_len. }
+         rewrite H1 in H0. now rewrite H0.
+Qed.
+
+Lemma forallb_eqb_refl: forall a, forallb2 eq_carry_lit (lit_to_carry a) a = true.
+Proof. intro a.
+       induction a; intros.
+       - now simpl.
+       - simpl. rewrite IHa. now case_eq (Lit.is_pos a ); rewrite Int63Axioms.eqb_refl.
+Qed. 
+
+Lemma zextend_interp_len: forall bs1 bsres (i: nat),
+                           check_zextend bs1 bsres i = true ->
+                           length bsres = (length bs1 + i)%nat.
+Proof. intro bs1.
+       induction bs1; intros.
+       - simpl in *. unfold check_zextend in H.
+         case_eq (forallb2 eq_carry_lit (lit_to_carry (zextend_lit [] i)) bsres); intros.
+         apply prop_eq_carry_lit2 in H0.
+         rewrite prop_interp_carry3 in H0. 
+         assert (length (map (Lit.interp rho) (zextend_lit [] i)) = length (map (Lit.interp rho) bsres)).
+         { now rewrite H0. }
+         rewrite !map_length in H1. unfold zextend_lit in H1. now rewrite length_empty_ext in H1.
+         rewrite H0 in H; now contradict H.
+       - simpl. unfold check_zextend in H.
+         case_eq ( forallb2 eq_carry_lit (lit_to_carry (zextend_lit (a :: bs1) i)) bsres); intros.
+         apply prop_eq_carry_lit2 in H0.
+         rewrite prop_interp_carry3 in H0.
+         assert (length (map (Lit.interp rho) (zextend_lit (a :: bs1) i)) = length (map (Lit.interp rho) bsres)).
+         { now rewrite H0. }
+         rewrite !map_length in H1. now rewrite zext_len in H1.
+         rewrite H0 in H; now contradict H.
+Qed.
+
+Lemma zextend_interp_main: forall bs1 bsres (i: nat),
+                           check_zextend bs1 bsres i = true ->
+                           Word.zext (ListToword (map (Lit.interp rho) bs1) (length bs1)) i  =
+                           ListToword (map (Lit.interp rho) bsres) ((length bs1) + i).
+Proof. intro bs1.
+       induction bs1 as [ | xbs1 xsbs1 IHbs1].
+       - intros. simpl.
+         unfold check_zextend in H. simpl in H.
+         case_eq (forallb2 eq_carry_lit
+          (lit_to_carry (zextend_lit [] i)) bsres).
+         intros.
+         apply prop_eq_carry_lit2 in H0.
+         rewrite prop_interp_carry3 in H0.
+         simpl in H0. unfold zext. rewrite <- H0. simpl. unfold zextend_lit in *.
+         now rewrite wzeron.
+         intros. rewrite H0 in H; now contradict H.
+       - intros. unfold RAWBITVECTOR_LIST.bv_zextn, check_zextend in H.
+         case_eq (
+          forallb2 eq_carry_lit
+          (lit_to_carry
+             (zextend_lit (xbs1 :: xsbs1) i))
+          bsres); intros.
+         apply prop_eq_carry_lit2 in H0.
+         rewrite prop_interp_carry3 in H0.
+         simpl in H0. simpl.
+
+         unfold zext in *.
+         specialize (@helper_strong (map (Lit.interp rho) xsbs1) 
+         (Lit.interp rho xbs1) ); intros. rewrite !map_length in H1. rewrite H1. simpl.
+         rewrite <- H0. rewrite zext_cons.
+         specialize (@helper_strong (map (Lit.interp rho) (zextend_lit xsbs1 i)) 
+         (Lit.interp rho xbs1) ); intros. rewrite !map_length in H2. rewrite zext_len in H2.
+         rewrite H2. 
+         
+         rewrite (@IHbs1 (zextend_lit xsbs1 i) i). reflexivity.
+         unfold check_zextend. now rewrite forallb_eqb_refl.
+         rewrite H0 in H; now contradict H.
+Qed.
+
+Lemma valid_check_bbZextend s pos lres : C.valid rho (check_bbZextend s pos lres).
+Proof.
+      unfold check_bbZextend.
+      case_eq (S.get s pos); [intros _|intros l1 [ |l] Heq1]; try now apply C.interp_true.
+      case_eq (Lit.is_pos l1); intro Heq2; simpl; try now apply C.interp_true.
+      case_eq (Lit.is_pos lres); intro Heq3; simpl; try now apply C.interp_true.
+      case_eq (t_form .[ Lit.blit l1]); try (intros; now apply C.interp_true). intros a1 bs1 Heq4.
+      case_eq (t_form .[ Lit.blit lres]); try (intros; now apply C.interp_true).
+      intros a bsres Heq5.
+      case_eq (t_atom .[ a]); try (intros; now apply C.interp_true).
+      intros [ | | | | | | ]  a1'  Heq6; try (intros; now apply C.interp_true).
+      (* BVzextend *)
+    - case_eq ((a1 == a1')); simpl; intros Heq7; try (now apply C.interp_true).
+        case_eq (
+            check_zextend bs1 bsres i && ((Datatypes.length bs1) =? n)%nat
+        ); simpl; intros Heq8; try (now apply C.interp_true).
+
+        unfold C.valid. simpl. rewrite orb_false_r.
+        unfold Lit.interp. rewrite Heq3.
+        unfold Var.interp.
+        rewrite wf_interp_form; trivial. rewrite Heq5. simpl.
+
+        apply Word.weqb_true_iff.
+
+        generalize wt_t_atom. unfold Atom.wt. unfold is_true.
+        rewrite PArray.forallbi_spec;intros.
+
+        pose proof (H a). 
+        assert (a < PArray.length t_atom).
+        { apply PArray.get_not_default_lt. rewrite def_t_atom. rewrite Heq6. easy. }
+        specialize (@H0 H1). rewrite Heq6 in H0. simpl in H0.
+        rewrite !andb_true_iff in H0. destruct H0.
+
+        unfold get_type' in H0. unfold v_type in H0.
+        case_eq (t_interp .[ a]).
+        intros v_typea v_vala Htia. rewrite Htia in H0.
+        case_eq (v_typea);  intros; rewrite H3 in H0; try (now contradict H0).
+        rename H0 into Hv.
+
+        generalize (Hs s pos). intros HSp. unfold C.valid in HSp. rewrite Heq1 in HSp.
+        unfold C.interp in HSp. unfold existsb in HSp. rewrite orb_false_r in HSp.
+        unfold Lit.interp in HSp. rewrite Heq2 in HSp. unfold Var.interp in HSp.
+        rewrite rho_interp in HSp. rewrite Heq4 in HSp. simpl in HSp.
+
+        apply Word.weqb_true_iff in HSp.
+
+        unfold get_type' in H2. unfold v_type in H2.
+        case_eq (t_interp .[ a1']).
+          intros v_typea1 v_vala1 Htia1. rewrite Htia1 in H2.
+        rewrite Atom.t_interp_wf in Htia1; trivial.
+        unfold apply_binop.
+        apply Typ.eqb_spec in H2.
+
+        (** case a1 = a1' **)
+        rewrite eqb_spec in Heq7; rewrite Heq7 in *.
+
+        (* interp_form_hatom_bv a = 
+                interp_bv t_i (interp_atom (t_atom .[a])) *)
+        assert (interp_form_hatom_word a = 
+                interp_word t_i (interp_atom (t_atom .[a]))).
+        {
+          rewrite !Atom.t_interp_wf in Htia; trivial.
+          rewrite Htia.
+          unfold Atom.interp_form_hatom_word.
+          unfold Atom.interp_hatom.
+          rewrite !Atom.t_interp_wf; trivial.
+          rewrite Htia. easy.
+        }
+
+        rewrite H0. rewrite Heq6. simpl.
+        unfold interp_word. unfold apply_unop.
+
+        rewrite !Atom.t_interp_wf; trivial.
+
+        revert v_vala1 Htia1. rewrite H2.
+        intros v_vala1 Htia1.
+        rewrite Htia1.
+        rewrite !Typ.cast_refl.
+        unfold Bval.
+
+        assert (H100: ( (Datatypes.length (map (Lit.interp rho) bsres))) = (n + i)%nat). 
+        { 
+           rewrite andb_true_iff in Heq8.
+           destruct Heq8 as (Heq8a, Heq8b).
+           rewrite map_length.
+           apply zextend_interp_len in Heq8a.
+           rewrite Nat.eqb_eq in Heq8b.
+           now rewrite Heq8b in Heq8a.
+        }
+
+        rewrite H100.
+        rewrite Typ.cast_refl. intros.
+        simpl.
+
+        (* interp_form_hatom_bv a1' = 
+                interp_bv t_i (interp_atom (t_atom .[a1'])) *)
+        assert (interp_form_hatom_word a1' = 
+                interp_word t_i (interp_atom (t_atom .[a1']))).
+        {
+          rewrite !Atom.t_interp_wf in Htia; trivial.
+          rewrite Htia1.
+          unfold Atom.interp_form_hatom_word.
+          unfold Atom.interp_hatom.
+          rewrite !Atom.t_interp_wf; trivial.
+          rewrite Htia1. easy.
+        }
+
+        rewrite H4 in HSp.
+        unfold interp_word in HSp.
+        rewrite Htia1 in HSp.
+        unfold interp_word in HSp. 
+
+        revert HSp.
+
+        assert (H101: ((Datatypes.length (map (Lit.interp rho) bs1))) = n).
+        {
+           rewrite andb_true_iff in Heq8.
+           destruct Heq8 as (Heq8a, Heq8b).
+           rewrite map_length.
+           now rewrite Nat.eqb_eq in Heq8b.
+        }
+
+        rewrite H101.
+        rewrite Typ.cast_refl. intros.
+        simpl.
+
+        rewrite HSp. simpl. unfold zext.
+        rewrite andb_true_iff in Heq8.
+        destruct Heq8 as (Heq8a, Heq8b).
+        rewrite map_length in H101. rewrite <- H101.
+        now apply zextend_interp_main.
+Qed.
+
 
 Lemma check_add_bvadd_length: forall bs1 bs2 bsres c,
   let n := length bsres in
@@ -6865,251 +7158,9 @@ Proof.
         rewrite H101 in H5. now apply H5.
 Qed.
 
-Lemma zextend_interp_zero: forall a, RAWBITVECTOR_LIST.zextend (map (Lit.interp rho) a) O =
-(map (Lit.interp rho) (zextend_lit a 0)).
-Proof. now simpl. Qed.
 
-Lemma zextend_interp_empty: forall i, RAWBITVECTOR_LIST.zextend (map (Lit.interp rho) []) i =
-map (Lit.interp rho) (zextend_lit [] i).
-Proof. simpl. intro i.
-       induction i.
-       - intros. now simpl.
-       - intros. simpl.
-         unfold RAWBITVECTOR_LIST.zextend in *.
-         simpl. rewrite IHi.
-         assert (Lit.interp rho Lit._false = false).
-           { specialize (Lit.interp_false rho wf_rho). intros.
-              rewrite <- not_true_iff_false.
-              unfold not in *.
-              intros. now apply H. }
-        now rewrite H.
- Qed.
 
-Lemma zextend_interp_all: forall a i, RAWBITVECTOR_LIST.zextend (map (Lit.interp rho) a) i =
-map (Lit.interp rho) (zextend_lit a i).
-Proof. intro a.
-       induction a as [ | xa xsa IHa].
-       - intros. simpl.
-         induction i.
-         + intros. now simpl.
-         + intros. unfold RAWBITVECTOR_LIST.zextend in *.
-           simpl. rewrite IHi.
-           assert (Lit.interp rho Lit._false = false).
-           { specialize (Lit.interp_false rho wf_rho). intros.
-              rewrite <- not_true_iff_false.
-              unfold not in *.
-              intros. now apply H. }
-           now rewrite H.
-        - intros. 
-          induction i.
-          + now simpl.
-          + unfold RAWBITVECTOR_LIST.zextend, zextend_lit in *.
-            simpl in *. rewrite <- IHi.
-           assert (Lit.interp rho Lit._false = false).
-           { specialize (Lit.interp_false rho wf_rho). intros.
-              rewrite <- not_true_iff_false.
-              unfold not in *.
-              intros. now apply H. }
-           now rewrite H.
-Qed.
 
-Lemma zextend_interp_main: forall bs1 bsres (n i: N),
-                           check_zextend bs1 bsres i = true ->
-                           @RAWBITVECTOR_LIST.bv_zextn n i
-                             (map (Lit.interp rho) bs1) = map (Lit.interp rho) bsres.
-Proof. intro bs1.
-       induction bs1 as [ | xbs1 xsbs1 IHbs1].
-       - intros. simpl.
-         unfold check_zextend in H. simpl in H.
-         case_eq (forallb2 eq_carry_lit
-          (lit_to_carry (zextend_lit [] (N.to_nat i))) bsres).
-         intros.
-         apply prop_eq_carry_lit2 in H0.
-         rewrite prop_interp_carry3 in H0.
-         simpl in H0.
-         unfold RAWBITVECTOR_LIST.bv_zextn.
-         now rewrite zextend_interp_empty.
-         intros. rewrite H0 in H. now contradict H0.
-       - intros. unfold RAWBITVECTOR_LIST.bv_zextn, check_zextend in H.
-         case_eq (
-          forallb2 eq_carry_lit
-          (lit_to_carry
-             (zextend_lit (xbs1 :: xsbs1) (N.to_nat i)))
-          bsres); intros.
-         apply prop_eq_carry_lit2 in H0.
-         rewrite prop_interp_carry3 in H0.
-         simpl in H0. simpl.
-
-         unfold RAWBITVECTOR_LIST.bv_zextn in *.
-         case_eq (N.to_nat i). intros. rewrite H1 in H0.
-         now simpl in *.
-         intros. rewrite H1 in H0.
-         rewrite <- H0.
-         rewrite <- zextend_interp_all.
-         simpl.
-         assert (Lit.interp rho Lit._false = false).
-         { specialize (Lit.interp_false rho wf_rho). intros.
-            rewrite <- not_true_iff_false.
-            unfold not in *.
-            intros. now apply H2. }
-         reflexivity.
-
-         rewrite H0 in H. now contradict H.
-Qed.
-
-Lemma valid_check_bbZextend pos lres : C.valid rho (check_bbZextend pos lres).
-Proof.
-      unfold check_bbZextend.
-      case_eq (S.get s pos); [intros _|intros l1 [ |l] Heq1]; try now apply C.interp_true.
-      case_eq (Lit.is_pos l1); intro Heq2; simpl; try now apply C.interp_true.
-      case_eq (Lit.is_pos lres); intro Heq3; simpl; try now apply C.interp_true.
-      case_eq (t_form .[ Lit.blit l1]); try (intros; now apply C.interp_true). intros a1 bs1 Heq4.
-      case_eq (t_form .[ Lit.blit lres]); try (intros; now apply C.interp_true).
-      intros a bsres Heq5.
-      case_eq (t_atom .[ a]); try (intros; now apply C.interp_true).
-      intros [ | | | | | | | | | | ]  a1'  Heq6; try (intros; now apply C.interp_true).
-      (* BVzextend *)
-    - case_eq ((a1 == a1')); simpl; intros Heq7; try (now apply C.interp_true).
-        case_eq (
-            check_zextend bs1 bsres i && (N.of_nat (Datatypes.length bs1) =? n)%N
-        ); simpl; intros Heq8; try (now apply C.interp_true).
-
-        unfold C.valid. simpl. rewrite orb_false_r.
-        unfold Lit.interp. rewrite Heq3.
-        unfold Var.interp.
-        rewrite wf_interp_form; trivial. rewrite Heq5. simpl.
-
-        apply BITVECTOR_LIST.bv_eq_reflect.
-
-        generalize wt_t_atom. unfold Atom.wt. unfold is_true.
-        rewrite PArray.forallbi_spec;intros.
-
-        pose proof (H a). 
-        assert (a < PArray.length t_atom).
-        { apply PArray.get_not_default_lt. rewrite def_t_atom. rewrite Heq6. easy. }
-        specialize (@H0 H1). rewrite Heq6 in H0. simpl in H0.
-        rewrite !andb_true_iff in H0. destruct H0.
-
-        unfold get_type' in H0. unfold v_type in H0.
-        case_eq (t_interp .[ a]).
-        intros v_typea v_vala Htia. rewrite Htia in H0.
-        case_eq (v_typea);  intros; rewrite H3 in H0; try (now contradict H0).
-        rename H0 into Hv.
-
-        generalize (Hs pos). intros HSp. unfold C.valid in HSp. rewrite Heq1 in HSp.
-        unfold C.interp in HSp. unfold existsb in HSp. rewrite orb_false_r in HSp.
-        unfold Lit.interp in HSp. rewrite Heq2 in HSp. unfold Var.interp in HSp.
-        rewrite rho_interp in HSp. rewrite Heq4 in HSp. simpl in HSp.
-
-        apply BITVECTOR_LIST.bv_eq_reflect in HSp.
-
-        unfold get_type' in H2. unfold v_type in H2.
-        case_eq (t_interp .[ a1']).
-          intros v_typea1 v_vala1 Htia1. rewrite Htia1 in H2.
-        rewrite Atom.t_interp_wf in Htia1; trivial.
-        unfold apply_binop.
-        apply Typ.eqb_spec in H2.
-
-        (** case a1 = a1' **)
-        rewrite eqb_spec in Heq7; rewrite Heq7 in *.
-
-        (* interp_form_hatom_bv a = 
-                interp_bv t_i (interp_atom (t_atom .[a])) *)
-        assert (interp_form_hatom_bv a = 
-                interp_bv t_i (interp_atom (t_atom .[a]))).
-        {
-          rewrite !Atom.t_interp_wf in Htia; trivial.
-          rewrite Htia.
-          unfold Atom.interp_form_hatom_bv.
-          unfold Atom.interp_hatom.
-          rewrite !Atom.t_interp_wf; trivial.
-          rewrite Htia. easy.
-        }
-
-        rewrite H0. rewrite Heq6. simpl.
-        unfold interp_bv. unfold apply_unop.
-
-        rewrite !Atom.t_interp_wf; trivial.
-
-        revert v_vala1 Htia1. rewrite H2.
-        intros v_vala1 Htia1.
-        rewrite Htia1.
-        rewrite !Typ.cast_refl.
-        unfold Bval.
-
-        assert (H100: (N.of_nat (Datatypes.length (map (Lit.interp rho) bsres))) = (i + n)%N).
-        {
-           rewrite andb_true_iff in Heq8.
-           destruct Heq8 as (Heq8a, Heq8b).
-           rewrite map_length.
-           specialize (@zextend_interp_main bs1 bsres n i).
-           intros.
-           apply H4 in Heq8a.
-           unfold RAWBITVECTOR_LIST.bv_zextn in Heq8a.
-           assert (length (RAWBITVECTOR_LIST.zextend (map (Lit.interp rho) bs1) (N.to_nat i)) 
-           = length (map (Lit.interp rho) bsres)).
-           { now rewrite Heq8a. }
-           rewrite RAWBITVECTOR_LIST.length_zextend, !map_length in H5.
-           apply (f_equal (N.of_nat)) in H5.
-           rewrite <- H5.
-           
-           rewrite N.eqb_eq in Heq8b.
-           apply (f_equal (N.to_nat)) in Heq8b.
-           rewrite Nat2N.id in Heq8b.
-           rewrite Heq8b. lia.
-        }
-
-        unfold BITVECTOR_LIST.of_bits, RAWBITVECTOR_LIST.of_bits.
-
-        generalize ( BITVECTOR_LIST.of_bits_size (map (Lit.interp rho) bsres)).
-
-        rewrite H100.
-        rewrite Typ.cast_refl. intros.
-        simpl.
-
-        (* interp_form_hatom_bv a1' = 
-                interp_bv t_i (interp_atom (t_atom .[a1'])) *)
-        assert (interp_form_hatom_bv a1' = 
-                interp_bv t_i (interp_atom (t_atom .[a1']))).
-        {
-          rewrite !Atom.t_interp_wf in Htia; trivial.
-          rewrite Htia1.
-          unfold Atom.interp_form_hatom_bv.
-          unfold Atom.interp_hatom.
-          rewrite !Atom.t_interp_wf; trivial.
-          rewrite Htia1. easy.
-        }
-
-        rewrite H4 in HSp.
-        unfold interp_bv in HSp.
-        rewrite Htia1 in HSp.
-        unfold interp_bv in HSp. 
-
-        revert HSp.
-
-        assert (H101: (N.of_nat (Datatypes.length (map (Lit.interp rho) bs1))) = n).
-        {
-           rewrite andb_true_iff in Heq8.
-           destruct Heq8 as (Heq8a, Heq8b).
-           rewrite map_length.
-           now rewrite N.eqb_eq in Heq8b.
-        }
-
-        unfold BITVECTOR_LIST.of_bits, RAWBITVECTOR_LIST.of_bits.
-
-        generalize ( BITVECTOR_LIST.of_bits_size (map (Lit.interp rho) bs1)).
-
-        rewrite H101.
-        rewrite Typ.cast_refl. intros.
-        simpl.
-
-        rewrite HSp. simpl.
-        unfold BITVECTOR_LIST.bv_zextn.
-        apply eq_rec. simpl.
-        rewrite andb_true_iff in Heq8.
-        destruct Heq8 as (Heq8a, Heq8b).
-        now apply zextend_interp_main.
-Qed.    
 
 Lemma sextend_interp_zero: forall a, RAWBITVECTOR_LIST.sextend (map (Lit.interp rho) a) O =
 (map (Lit.interp rho) (sextend_lit a 0)).
